fstar/MLS.Test.FromExt.KeySchedule.fst
@@ -18,7 +18,7 @@ let gen_group_context group_id epoch inp =
   let group_id = hex_string_to_bytes group_id in
   let tree_hash = hex_string_to_bytes inp.tree_hash in
   let confirmed_transcript_hash = hex_string_to_bytes inp.confirmed_transcript_hash in
-  if length group_id <= 255 && epoch < (pow2 64) && length tree_hash <= 255 && length confirmed_transcript_hash <= 255 then (
+  if length group_id < pow2 30 && epoch < (pow2 64) && length tree_hash < pow2 30 && length confirmed_transcript_hash < pow2 30 then (
     bytes_length_nil #bytes ps_extension_nt;
     (ps_to_pse ps_group_context_nt).serialize_exact ({
       group_id = group_id;
